src/program_proof/mvcc/mvcc_proof.v
@@ -15,4 +15,6 @@ From Perennial.program_proof.mvcc Require Export
      tuple_append_version tuple_kill_version tuple_read_version
      tuple_remove_versions tuple_own tuple_free tuple_write_lock
      (* examples *)
-     examples_rsvkey examples_counter.
+     examples_rsvkey examples_counter
+	 (* tpcc *)
+	 tpcc_prelude tpcc_customer.
