src/program_proof/mvcc/tpcc_customer.v
@@ -1,0 +1,478 @@
+From Perennial.program_proof.mvcc Require Import tpcc_prelude.
+
+Section program.
+Context `{!heapGS Σ}.
+
+(**
+ * Application-specific point-tos are defined in terms of [txnmaps_ptsto] and [dbmaps_ptsto].
+ *)
+
+(* Resources and operations on the Customer table. *)
+Lemma struct_ty_customer_unfold :
+  struct.t Customer = (uint64T * (uint64T * (slice.T byteT * unitT)))%ht.
+Proof. reflexivity. Qed.
+
+Definition customer_record_to_val (cid : u64) (cwid : u64) (clast : Slice.t) :=
+  (#cid, (#cwid, (to_val clast, #())))%V.
+
+Definition customer_tbl_txnpt (τ : gname) (tplid : u64) (data : u64 * u64 * (list u8)) :=
+  txnmaps_ptsto τ (U64 0) (u64_le tplid) (Value (u64_le data.1.1 ++ u64_le data.1.2 ++ data.2)).
+
+Definition customer_tbl_dbpt (τ : gname) (tplid : u64) q (data : u64 * u64 * (list u8)) :=
+  dbmaps_ptsto τ (U64 0) (u64_le tplid) q (Value (u64_le data.1.1 ++ u64_le data.1.2 ++ data.2)).
+
+Theorem wp_readCustomer txn tplid cid cwid clast tid view γ τ :
+  {{{ own_txn txn tid view γ τ ∗ customer_tbl_txnpt τ tplid (cid, cwid, clast) }}}
+    readCustomer #txn #tplid
+  {{{ (clastS : Slice.t), RET (customer_record_to_val cid cwid clastS);
+      own_txn txn tid view γ τ ∗ customer_tbl_txnpt τ tplid (cid, cwid, clast) ∗
+      is_slice_small clastS byteT 1 clast
+  }}}.
+Proof.
+  iIntros (Φ) "[Htxn Hpt] HΦ".
+  wp_call.
+
+  (***********************************************************)
+  (* var k = make([]byte, 0, 8)                              *)
+  (* k = marshal.WriteInt(k, tplid)                          *)
+  (***********************************************************)
+  wp_apply wp_NewSliceWithCap; first word.
+  iIntros (kPtr) "HkS".
+  replace (int.nat 0) with 0%nat by word. rewrite replicate_0.
+  wp_apply wp_ref_to; first by auto.
+  iIntros (kRef) "HkRef".
+  wp_load.
+  wp_apply (wp_WriteInt with "HkS").
+  iIntros (kS) "HkS /=".
+  wp_store.
+  
+  (***********************************************************)
+  (* v, _ := txn.Read(MAPID_CUSTOMER_TBL, k)                 *)
+  (***********************************************************)
+  wp_load.
+  wp_apply (wp_txn__Read with "[$Htxn $Hpt $HkS]").
+  set v' := (u64_le _ ++ u64_le _ ++ _).
+  iIntros (vS found v) "(Htxn & Hpt & HkS & HvS & %Hret)".
+  destruct found eqn:Efound; last by inversion Hret.
+  wp_pures.
+
+  (***********************************************************)
+  (* cid, v1 := marshal.ReadInt(v)                           *)
+  (* cwid, clast := marshal.ReadInt(v1)                      *)
+  (* return Customer {                                       *)
+  (*     C_ID : cid,                                         *)
+  (*     C_W_ID : cwid,                                      *)
+  (*     C_LAST : clast,                                     *)
+  (* }                                                       *)
+  (***********************************************************)
+  simpl in Hret. inversion Hret. subst v'.
+  iDestruct (is_slice_to_small with "HvS") as "HvS".
+  wp_apply (wp_ReadInt with "HvS").
+  iIntros (vS') "HvS'".
+  wp_pures.
+  wp_apply (wp_ReadInt with "HvS'").
+  iIntros (vS'') "HvS''".
+  wp_pures.
+  iApply "HΦ".
+  by iFrame.
+Qed.
+
+(* Resources and operations on the Customer index. *)
+Definition customer_idx_txnpt (τ : gname) (cid cwid : u64) (tplid : u64) :=
+  txnmaps_ptsto τ (U64 1) ((u64_le cid) ++ (u64_le cwid)) (Value (u64_le tplid)).
+
+Definition customer_idx_txnpt_nil (τ : gname) (cid cwid : u64) :=
+  txnmaps_ptsto τ (U64 1) ((u64_le cid) ++ (u64_le cwid)) Nil.
+
+Definition customer_idx_dbpt (τ : gname) (cid cwid : u64) q (tplid : u64) :=
+  dbmaps_ptsto τ (U64 1) ((u64_le cid) ++ (u64_le cwid)) q (Value (u64_le tplid)).
+
+Definition customer_idx_dbpt_nil (τ : gname) (cid cwid : u64) q :=
+  dbmaps_ptsto τ (U64 1) ((u64_le cid) ++ (u64_le cwid)) q Nil.
+
+Theorem wp_findCusomterByCID txn cid cwid tid tplid view γ τ :
+  {{{ own_txn txn tid view γ τ ∗ customer_idx_txnpt τ cid cwid tplid }}}
+    findCustomerByCID #txn #cid #cwid
+  {{{ RET (#tplid, #true);
+      own_txn txn tid view γ τ ∗ customer_idx_txnpt τ cid cwid tplid
+  }}}.
+Proof.
+  iIntros (Φ) "[Htxn Hpt] HΦ".
+  wp_call.
+
+  (***********************************************************)
+  (* var k = make([]byte, 0, 16)                             *)
+  (* k = marshal.WriteInt(k, cid)                            *)
+  (* k = marshal.WriteInt(k, cwid)                           *)
+  (***********************************************************)
+  wp_apply wp_NewSliceWithCap; first word.
+  iIntros (kPtr) "HkS".
+  replace (int.nat 0) with 0%nat by word. rewrite replicate_0.
+  wp_apply wp_ref_to; first by auto.
+  iIntros (kRef) "HkRef".
+  wp_load.
+  wp_apply (wp_WriteInt with "HkS").
+  iIntros (kS) "HkS /=".
+  wp_store.
+  wp_load.
+  wp_apply (wp_WriteInt with "HkS").
+  iIntros (kS') "HkS'".
+  wp_store.
+
+  (***********************************************************)
+  (* v, ok := txn.Read(MAPID_CUSTOMER_IDX_CID, k)            *)
+  (* if !ok {                                                *)
+  (*     return 0, false                                     *)
+  (* }                                                       *)
+  (***********************************************************)
+  wp_load.
+  wp_apply (wp_txn__Read with "[$Htxn $Hpt $HkS']").
+  set k := (u64_le _ ++ u64_le _).
+  iIntros (vS found v) "(Htxn & Hpt & HkS & HvS & %Hret)".
+  destruct found eqn:Efound; last by inversion Hret.
+  wp_pures.
+
+  (***********************************************************)
+  (* tplid, _ := marshal.ReadInt(v)                          *)
+  (* return tplid, true                                      *)
+  (***********************************************************)
+  simpl in Hret. inversion Hret. subst v.
+  iDestruct (is_slice_to_small with "HvS") as "HvS".
+  wp_apply (wp_ReadInt with "HvS").
+  iIntros (vS') "HvS'".
+  wp_pures.
+  iApply "HΦ".
+  by iFrame.
+Qed.
+
+Theorem wp_findCusomterByCID_nil txn cid cwid tid view γ τ :
+  {{{ own_txn txn tid view γ τ ∗ customer_idx_txnpt_nil τ cid cwid }}}
+    findCustomerByCID #txn #cid #cwid
+  {{{ RET (#(U64 0), #false);
+      own_txn txn tid view γ τ ∗ customer_idx_txnpt_nil τ cid cwid
+  }}}.
+Proof.
+  iIntros (Φ) "[Htxn Hpt] HΦ".
+  wp_call.
+
+  (***********************************************************)
+  (* var k = make([]byte, 0, 16)                             *)
+  (* k = marshal.WriteInt(k, cid)                            *)
+  (* k = marshal.WriteInt(k, cwid)                           *)
+  (***********************************************************)
+  wp_apply wp_NewSliceWithCap; first word.
+  iIntros (kPtr) "HkS".
+  replace (int.nat 0) with 0%nat by word. rewrite replicate_0.
+  wp_apply wp_ref_to; first by auto.
+  iIntros (kRef) "HkRef".
+  wp_load.
+  wp_apply (wp_WriteInt with "HkS").
+  iIntros (kS) "HkS /=".
+  wp_store.
+  wp_load.
+  wp_apply (wp_WriteInt with "HkS").
+  iIntros (kS') "HkS'".
+  wp_store.
+
+  (***********************************************************)
+  (* v, ok := txn.Read(MAPID_CUSTOMER_IDX_CID, k)            *)
+  (* if !ok {                                                *)
+  (*     return 0, false                                     *)
+  (* }                                                       *)
+  (***********************************************************)
+  wp_load.
+  wp_apply (wp_txn__Read with "[$Htxn $Hpt $HkS']").
+  set k := (u64_le _ ++ u64_le _).
+  iIntros (vS found v) "(Htxn & Hpt & HkS & HvS & %Hret)".
+  destruct found eqn:Efound; first inversion Hret.
+  wp_pures.
+  iApply "HΦ".
+  by iFrame.
+Qed.
+
+(* Query the Customer table with its index. *)
+Theorem wp_SelectCusomterByCID txn cid cwid (cref : loc) clast tid tplid view γ τ :
+  {{{ own_txn txn tid view γ τ ∗ 
+      customer_idx_txnpt τ cid cwid tplid ∗ customer_tbl_txnpt τ tplid (cid, cwid, clast) ∗
+      (∃ cid' cwid' clast', cref ↦[structTy Customer] (customer_record_to_val cid' cwid' clast'))
+  }}}
+    SelectCustomerByCID #txn #cid #cwid #cref
+  {{{ (clastS : Slice.t), RET #true;
+      own_txn txn tid view γ τ ∗
+      customer_idx_txnpt τ cid cwid tplid ∗ customer_tbl_txnpt τ tplid (cid, cwid, clast) ∗
+      cref ↦[Customer :: "C_ID"] #cid ∗ cref ↦[Customer :: "C_W_ID"] #cwid ∗
+      cref ↦[Customer :: "C_LAST"] (to_val clastS) ∗ is_slice_small clastS byteT 1 clast
+  }}}.
+Proof.
+  iIntros (Φ) "(Htxn & Hidxpt & Htblpt & Hc) HΦ".
+  wp_call.
+
+  (***********************************************************)
+  (* tplid, found := findCustomerByCID(txn, cid, cwid)       *)
+  (* if !found {                                             *)
+  (*     return false                                        *)
+  (* }                                                       *)
+  (***********************************************************)
+  wp_apply (wp_findCusomterByCID with "[$Htxn $Hidxpt]").
+  iIntros "[Htxn Hidxpt]".
+  wp_pures.
+  
+  (***********************************************************)
+  (* customer := readCustomer(txn, tplid)                    *)
+  (* *cref = customer                                        *)
+  (***********************************************************)
+  wp_apply (wp_readCustomer with "[$Htxn $Htblpt]").
+  iIntros (clastS) "(Htxn & Htblpt & HclastS)".
+  wp_pures.
+  iDestruct "Hc" as (cid' cwid' clast') "Hc".
+  iDestruct (struct_fields_split with "Hc") as "Hc".
+  iNamed "Hc".
+  do 3 wp_storeField.
+
+  (***********************************************************)
+  (* return true                                             *)
+  (***********************************************************)
+  iApply "HΦ".
+  by iFrame.
+Qed.
+
+Theorem wp_SelectCusomterByCID_nil txn cid cwid (cref : loc) tid view γ τ :
+  {{{ own_txn txn tid view γ τ ∗ customer_idx_txnpt_nil τ cid cwid }}}
+    SelectCustomerByCID #txn #cid #cwid #cref
+  {{{ RET #false;
+      own_txn txn tid view γ τ ∗ customer_idx_txnpt_nil τ cid cwid
+  }}}.
+Proof.
+  iIntros (Φ) "[Htxn Hidxpt] HΦ".
+  wp_call.
+
+  (***********************************************************)
+  (* tplid, found := findCustomerByCID(txn, cid, cwid)       *)
+  (* if !found {                                             *)
+  (*     return false                                        *)
+  (* }                                                       *)
+  (***********************************************************)
+  wp_apply (wp_findCusomterByCID_nil with "[$Htxn $Hidxpt]").
+  iIntros "[Htxn Hidxpt]".
+  wp_pures.
+  iApply "HΦ".
+  by iFrame.
+Qed.
+
+(* Functions below are not the interface of this file. *)
+
+(**
+ * TODO: We're forcing full ownership of [customer_idx_dbpt] and
+ * [customer_tbl_dbpt].
+ * Maybe should define [dbmaps_ptstos_wr], which requires full
+ * ownership of each individual [dbmaps_ptsto]s, and
+ * [dbmaps_ptstos_rd] which requires only partial ownership, and prove
+ * [wp_txn__DoTxn_readonly] that uses the latter one.
+ *)
+Theorem wp_TxnSelectCusomterByCID txn cid cwid γ :
+  ⊢ {{{ own_txn_uninit txn γ }}}
+    <<< ∀∀ (tplid : u64) (clast : list u8),
+        customer_idx_dbpt γ cid cwid 1 tplid ∗ customer_tbl_dbpt γ tplid 1 (cid, cwid, clast)
+    >>>
+    TxnSelectCustomerByCID #txn #cid #cwid @ ⊤
+    <<< customer_idx_dbpt γ cid cwid 1 tplid ∗ customer_tbl_dbpt γ tplid 1 (cid, cwid, clast) >>>
+    {{{ (clastS : Slice.t), RET customer_record_to_val cid cwid clastS;
+        own_txn_uninit txn γ ∗ is_slice_small clastS byteT 1 clast
+    }}}.
+Proof.
+  iIntros (Φ) "!> Htxn HAU".
+  wp_call.
+
+  (***********************************************************)
+  (* var c Customer                                          *)
+  (* body := func(txn *Txn) bool {                           *)
+  (*     return selectCustomerByCID(txn, cid, cwid, &c)      *)
+  (* }                                                       *)
+  (* t.DoTxn(body)                                           *)
+  (* return c                                                *)
+  (***********************************************************)
+  wp_apply (wp_ref_of_zero); first by auto.
+  iIntros (cRef) "HcRef".
+  wp_pures.
+  set m : u64 -> list u8 -> dbmaps :=
+    λ (tplid : u64) (clast : list u8),
+      {[ (U64 1, u64_le cid ++ u64_le cwid) := Value (u64_le tplid) ]} ∪
+      {[ (U64 0, u64_le tplid) := Value (u64_le cid ++ u64_le cwid ++ clast) ]}.
+
+
+  (* Q: Can we automate converting [big_sepM] to individual points-tos? *)
+  iAssert (∀ (tplid : u64) (clast : list u8) (τ : gname),
+             txnmaps_ptstos τ (m tplid clast) ∗-∗
+             (customer_idx_txnpt τ cid cwid tplid ∗ customer_tbl_txnpt τ tplid (cid, cwid, clast))
+          )%I as "Htxnptsiff".
+  { iIntros (tplid clast τ).
+    subst m. unfold txnmaps_ptstos.
+    rewrite big_sepM_union; last first.
+    { apply map_disjoint_dom_2. set_solver. }
+    do 2 rewrite big_sepM_singleton.
+    iSplit; by iIntros.
+  }
+  iAssert (∀ (tplid : u64) (clast : list u8),
+             dbmaps_ptstos γ 1 (m tplid clast) ∗-∗
+             (customer_idx_dbpt γ cid cwid 1 tplid ∗ customer_tbl_dbpt γ tplid 1 (cid, cwid, clast))
+          )%I as "Hdbptsiff".
+  { iIntros (tplid clast).
+    subst m. unfold dbmaps_ptstos.
+    rewrite big_sepM_union; last first.
+    { apply map_disjoint_dom_2. set_solver. }
+    do 2 rewrite big_sepM_singleton.
+    iSplit; by iIntros.
+  }
+
+
+  set P := λ (r : dbmaps), ∃ (tplid : u64) (clast : list u8), r = m tplid clast.
+  set Ri := (∃ cid cwid clastS,
+                cRef ↦[structTy Customer] (customer_record_to_val cid cwid clastS))%I.
+  set Ra := (λ (_ : dbmaps), Ri)%I.
+  set Rc := (λ (r : dbmaps), ∃ (tplid : u64) (clast : list u8) (clastS : Slice.t),
+                ⌜r !! (U64 1, u64_le cid ++ u64_le cwid) = Some (Value (u64_le tplid)) ∧
+                 r !! (U64 0, u64_le tplid) = Some (Value (u64_le cid ++ u64_le cwid ++ clast))⌝ ∗
+                cRef ↦[structTy Customer] (customer_record_to_val cid cwid clastS) ∗
+                is_slice_small clastS byteT 1 clast)%I.
+  wp_apply (wp_txn__DoTxn_readonly _ _ P Rc Rc with "[$Htxn HcRef]").
+  { (* Transaction body. *)
+    clear Φ. unfold spec_body.
+    iIntros (tid r τ Φ) "(Htxn & %HP & Htxnpts) HΦ".
+    unfold P in HP. destruct HP as (tplid & clast & Hr).
+    rewrite {2} Hr.
+    iDestruct ("Htxnptsiff" with "Htxnpts") as "[Hidxpt Htblpt]".
+    wp_pures.
+    wp_apply (wp_SelectCusomterByCID with "[$Htxn Hidxpt Htblpt HcRef]").
+    { iFrame. rewrite /zero_val /=.
+      iExists (U64 0), (U64 0), Slice.nil.
+      iFrame.
+    }
+    iIntros (clastS) "(Htxn & Hidxpt & Htblpt & Hcid & Hcwid & Hclast & HclastS)".
+    iApply "HΦ".
+    iFrame.
+    iSplitL "Hidxpt Htblpt".
+    { rewrite Hr.
+      (* Q: WOW how does IPM pick the correct direction? *)
+      iDestruct ("Htxnptsiff" with "[$Hidxpt $Htblpt]") as "Htxnpts".
+      iFrame.
+    }
+    iAssert (Rc r)%I with "[-]" as "H".
+    { subst Rc.
+      simpl.
+      (* Q: How to stop simplifying [u64_le]? *)
+      iExists tplid, clast, clastS.
+      rewrite -struct_ty_customer_unfold struct_fields_split.
+      iFrame.
+      iPureIntro.
+      subst m. simpl in Hr.
+      split; last done.
+      split; subst r.
+      { apply lookup_union_Some_l. by rewrite lookup_singleton. }
+      { apply lookup_union_Some_r; last by rewrite lookup_singleton.
+        apply map_disjoint_dom_2.
+        set_solver.
+      }
+    }
+    iFrame.
+  }
+  iMod "HAU" as (tplid clast) "[[Hidxpt Htblpt] HAU]".
+  iModIntro.
+  iExists (m tplid clast).
+  iDestruct ("Hdbptsiff" with "[$Hidxpt $Htblpt]") as "Hdbpts".
+  iFrame.
+  iSplit.
+  { subst P. eauto. }
+  iIntros "Hdbpts".
+  iDestruct ("Hdbptsiff" with "Hdbpts") as "[Hidxpt Htblpt]".
+  iMod ("HAU" with "[$Hidxpt $Htblpt]") as "HΦ".
+  iIntros "!>" (ok) "[Htxn HR]".
+  wp_pures.
+  iAssert (Rc (m tplid clast))%I with "[HR]" as "HR".
+  { destruct ok; done. }
+  subst Rc.
+  iDestruct "HR" as (tplid' clast' clastS) "([%Hlookup1 %Hlookup2] & HcRef & HclastS)".
+  wp_load.
+  wp_pures.
+  iApply "HΦ".
+  replace clast' with clast; last first.
+  { subst m.
+    rewrite (lookup_union_Some_l _ _ _ (Value (u64_le tplid))) in Hlookup1; last first.
+    { by rewrite lookup_singleton. }
+    do 2 apply Some_inj in Hlookup1.
+    rewrite -Hlookup1 in Hlookup2.
+    rewrite (lookup_union_Some_r _ _ _ (Value (u64_le cid ++ u64_le cwid ++ clast))) in Hlookup2; last first.
+    { by rewrite lookup_singleton. }
+    { apply map_disjoint_dom_2. set_solver. }
+    do 2 apply Some_inj in Hlookup2.
+    set_solver.
+  }
+  by iFrame.
+Qed.
+
+Theorem wp_TxnSelectCusomterByCID_nil txn cid cwid γ :
+  ⊢ {{{ own_txn_uninit txn γ }}}
+    (* [x] is just a placeholder for missing notations. *)
+    <<< ∀∀ (x : u64), customer_idx_dbpt_nil γ cid cwid 1 >>>
+    TxnSelectCustomerByCID #txn #cid #cwid @ ⊤
+    <<< customer_idx_dbpt_nil γ cid cwid 1 >>>
+    {{{ RET (zero_val (struct.t Customer)); own_txn_uninit txn γ }}}.
+Proof.
+  iIntros (Φ) "!> Htxn HAU".
+  wp_call.
+
+  (***********************************************************)
+  (* var c Customer                                          *)
+  (* body := func(txn *Txn) bool {                           *)
+  (*     return selectCustomerByCID(txn, cid, cwid, &c)      *)
+  (* }                                                       *)
+  (* t.DoTxn(body)                                           *)
+  (* return c                                                *)
+  (***********************************************************)
+  wp_apply (wp_ref_of_zero); first by auto.
+  iIntros (cRef) "HcRef".
+  wp_pures.
+  set m : dbmaps := {[ (U64 1, u64_le cid ++ u64_le cwid) := Nil ]}.
+  set P := λ (r : dbmaps), r = m.
+  wp_apply (wp_txn__DoTxn_xres_readonly _ _ P with "[$Htxn]").
+  { (* Transaction body. *)
+    clear Φ. unfold spec_body.
+    iIntros (tid r τ Φ) "(Htxn & %HP & Hidxpt) HΦ".
+    unfold P in HP.
+    wp_pures.
+    unfold txnmaps_ptstos.
+    rewrite {2}HP big_sepM_singleton.
+    wp_apply (wp_SelectCusomterByCID_nil with "[$Htxn $Hidxpt]").
+    iIntros "[Htxn Hidxpt]".
+    iApply "HΦ".
+    rewrite HP big_sepM_singleton.
+    iFrame.
+  }
+  iMod "HAU".
+  iModIntro.
+  iDestruct "HAU" as (_) "[Hidxpt HAU]".
+  iExists m.
+  subst m.
+  rewrite /dbmaps_ptstos big_sepM_singleton.
+  iFrame.
+  iSplit; first done.
+  iIntros "Hidxpt".
+  iMod ("HAU" with "Hidxpt") as "HΦ".
+  iIntros "!>" (ok) "Htxn".
+  wp_load.
+  iApply "HΦ".
+  by iFrame.
+Qed.
+
+(**
+ * We need these invariants to use [SelectCusomterByCID]:
+ * 1. Index and table well-formedness
+ * 2. Index referential integrity 
+ *
+ * Invoking [SelectCusomterByCID]:
+ * 1. Open the invariant.
+ * 2. By index well-formedness, we can do a case analysis:
+ * 3-1. No such index entry -> use [wp_TxnSelectCusomterByCID_nil].
+ * 3-2. Index entry exists -> by referential integrity and table well-formedness -> use [wp_TxnSelectCusomterByCID].
+ *)
+
+End program.
